fix everything

Rustv/Rustv.thy
@@ -5,6 +5,8 @@ begin
 abbreviation "collect_tags_stack == BorrowStack.collect_tags"
 abbreviation "pop_tags_stack == BorrowStack.pop_tags"
 abbreviation "writable_stack == BorrowStack.writable"
+abbreviation "reborrow_comp_stack == BorrowStack.reborrow_comp"
+abbreviation "reborrow_stack == BorrowStack.reborrow"
 
 record globals_ram =
   memory :: "val list"
@@ -32,6 +34,7 @@ lemma wf_tags_update:
   assumes
     "wf_tags ts"
     "wf_reborrow stack"
+    "stack_finite stack"
   shows "wf_tags (ts[p := stack])"
   using assms set_update_subset_insert wf_tags_spec by fastforce
 
@@ -129,7 +132,8 @@ lemma pop_tags_wf_tags:
   using assms(1) apply (rule pop_tags_elims, simp add: Let_def)
   apply (rule wf_tags_update)
   using assms(4) apply simp
-  using assms dropWhile_stack_reborrow wf_tags_spec by simp
+  using assms dropWhile_stack_reborrow wf_tags_spec apply simp
+  using assms dropWhile_stack_finite wf_tags_spec by simp
 
 lemma hd_pop_tags:
   assumes
@@ -277,12 +281,13 @@ fun reborrow :: "ref_kind \<Rightarrow> tagged_ref \<Rightarrow> 'a globals_ram_
   "reborrow k r s =
     (let p = the_ptr (pointer r) in
     let t = new_tag s in
-    let tags = (tags s)[p := reborrow_comp k t (tag r) ((tags s) ! p)] in
+    let tags = (tags s)[p := reborrow_comp_stack k t (tag r) ((tags s) ! p)] in
     (\<lparr> pointer = pointer r, tag = t \<rparr>,  s\<lparr> tags := tags, issued_tags := t # issued_tags s \<rparr>))"
 
+declare BorrowStack.reborrow_comp.simps [simp del]
 fun_cases reborrow_elims: "reborrow k r s = (r', s')"
+declare BorrowStack.reborrow_comp.simps [simp]
 
-(*
 lemma collect_tags_stack_reborrow_subset:
   assumes
     "pop_tags_stack parent stack = popped"
@@ -300,20 +305,18 @@ lemma collect_tags_reborrow_subset:
   "\<lbrakk>the_ptr (pointer r) < length (tags s); reborrow k r s = (r', s')\<rbrakk> \<Longrightarrow> collect_tags (tags s') \<subseteq> {new_tag s} \<union> collect_tags (tags s)"
   apply (erule reborrow_elims)
   apply (simp add: Let_def del: reborrow_comp.simps)
-  using collect_tags_update_subset reborrow_comp_subset collect_tags_spec' nth_mem by blas
+  using collect_tags_update_subset reborrow_comp_subset collect_tags_spec' nth_mem by blast
 
 lemma collect_tags_reborrow_subset':
-  "\<lbrakk>the_ptr (pointer r) < length (tags s)\<rbrakk>
+  "\<lbrakk>the_ptr (pointer r) < length (tags s)\<rbrakk> 
   \<Longrightarrow> collect_tags (tags (snd (reborrow k r s))) \<subseteq> {new_tag s} \<union> collect_tags (tags s)"
   apply (simp add: Let_def del: reborrow_comp.simps)
-  using collect_tags_update_subset reborrow_comp_subset collect_tags_spec' nth_mem by blas
-*)
+  using collect_tags_update_subset reborrow_comp_subset collect_tags_spec' nth_mem by blast
 
 lemma reborrow_pointer: "reborrow k r s = (r', s') \<Longrightarrow> pointer r' = pointer r"
   apply (erule reborrow_elims)
   by (auto simp add: Let_def)
 
-(*
 lemma new_tag_collect:
   assumes
     "p < length ts"
@@ -332,69 +335,29 @@ proof -
   ultimately have "x \<in> {t'} \<union> collect_tags ts" by auto
   then show ?thesis using assms by auto
 qed
-*)
 
-lemma new_tag_collect:
-  assumes
-    "p < length ts"
-    "x \<in> collect_tags (ts[p := THE stack'. reborrow' k deriv orig (ts ! p) stack'])"
-      (is "x \<in> collect_tags (ts[p := ?stack'])")
-    "collect_tags ts \<subseteq> issued"
-    "x \<notin> issued"
-    "\<exists>stack'. reborrow' k deriv orig (ts ! p) stack'"
-  shows "x = deriv"
-proof -
-  have *: "x \<notin> collect_tags_stack (ts ! p)" using assms collect_tags_spec' nth_mem by blast
-  have "x \<in> collect_tags_stack ?stack' \<union> collect_tags ts"
-    using collect_tags_update_subset assms by blast
-  then have "x \<in> collect_tags_stack ?stack'"
-    using assms by auto
-  then have "x \<in> {deriv} \<union> collect_tags_stack (ts ! p)" using reborrow'_subset assms
-    by (metis insert_subset mk_disjoint_insert reborrow_unique the_equality)
-  then show ?thesis using * by auto
-qed
+lemma reborrow_update_heap': "\<lbrakk>wf_heap s; writable r s\<rbrakk> \<Longrightarrow> wf_heap (snd (reborrow k r s))"
+  apply (auto simp add: Let_def)
+   apply (rule wf_tags_update, auto)
+    apply (rule wf_reborrow_reborrow_comp, auto)
+     apply (simp add: wf_tags_spec)
+  using new_tag_notin_at apply fastforce
+   apply (rule stack_finite_reborrow, auto)
+   apply (rule dropWhile_stack_finite)
+   apply (simp add: wf_tags_spec)
+  using new_tag_collect by auto
 
-lemma ex_reborrow'_writable:
-  assumes
-    "wf_heap s"
-    "writable r s"
-    "the_ptr (pointer r) < length (tags s)"
-  shows "\<exists>!stack'. reborrow' k deriv (tag r) ((tags s) ! (the_ptr (pointer r))) stack'"
-  using BorrowStack.ex1_reborrow'_writable wf_tags_spec assms by auto
-
-lemma reborrow_update_heap':
-  assumes
-    "wf_heap s"
-    "writable r s"
-    "the_ptr (pointer r) < length (tags s)"
-  shows "wf_heap (snd (reborrow k r s))"
-  using assms apply (auto simp add: Let_def)
-   apply (rule wf_tags_update)
-    apply assumption
-   apply (rule wf_reborrow_reborrow')
-     apply (rule theI')
-     apply (auto simp add: ex_reborrow'_writable)
-  using wf_tags_spec apply auto[1]
-  sorry
-(*
-  using new_tag_notin_at apply fastforc
-  apply (rule new_tag_collect, auto)
-  using ex_reborrow'_writable assms by blast *)
-
-lemma reborrow_update_heap:
-  "\<lbrakk>wf_heap s; writable r s; the_ptr (pointer r) < length (tags s); reborrow k r s = (r', s')\<rbrakk> \<Longrightarrow> wf_heap s'"
+lemma reborrow_update_heap: "\<lbrakk>wf_heap s; writable r s; reborrow k r s = (r', s')\<rbrakk> \<Longrightarrow> wf_heap s'"
   using reborrow_update_heap' by (metis snd_conv)
 
 lemma reborrow_writable: "\<lbrakk>wf_heap s; writable r s; reborrow k r s = (r', s')\<rbrakk> \<Longrightarrow> writable r s'"
   apply (erule reborrow_elims)
-  apply (simp add: Let_def)
-  sorry
-(*
-  apply (rule writable_reborrow)
-     apply (rule theI')
-     apply (simp add: Rustv.ex_reborrow'_writable)
+  apply (simp add: Let_def del: BorrowStack.reborrow_comp.simps)
+  apply (rule writable_reborrow_comp)
+     apply blast
+    apply blast
   using wf_tags_spec nth_mem apply blast
-  using new_tag_notin_at by auto *)
+  using new_tag_notin_at by auto
 
 lemma reborrow_writable_derived:
   assumes
@@ -402,16 +365,12 @@ lemma reborrow_writable_derived:
     "writable r s"
     "reborrow k r s = (r', s')"
     "k = Unique \<or> k = SharedReadWrite"
-    "the_ptr (pointer r) < length (tags s)"
   shows "writable r' s'"
   using assms(3) apply (rule reborrow_elims)
-  using assms apply (simp add: Let_def)
-  sorry
-(*
-  apply (rule writable_reborrow_derived)
-     apply (rule theI')
-     apply (simp add: Rustv.ex_reborrow'_writable)
-  using wf_tags_spec by auto *)
+  using assms apply (simp add: Let_def del: BorrowStack.reborrow_comp.simps)
+  apply (rule writable_reborrow_comp_derived[of "tag r" "tags s ! the_ptr (pointer r)" k])
+  using wf_tags_spec apply auto[3]
+  using new_tag_notin_at by auto
 
 lemma lemma_for_write_ex1:
   assumes
